# New input pair0:
```java
    int year1 = 2020;
    int half1 = 1;
    int year2 = 2023;
    int year3 = 2023;
    int half3 = 1;
```
## Code to generate follow-up input0:
```java
    int year1 = 2020;
    int half1 = 1;
    int year2 = 2023;
    int year3 = year1;
    int half3 = half1;
```
Explanation: The inferred relation is that the result of `YearHalf.of(year1, half1).with(Year.of(year2))` should be equal to `YearHalf.of(year3, half3)`. Since `year1` and `year2` are the same, the result of `Year.of(year2)` is also the same as `Year.of(year1)`, so the inferred relation is satisfied.

# New input pair1:
```java
    int year1 = 1990;
    int half1 = 2;
    int year2 = 1995;
    int year3 = 1995;
    int half3 = 2;
```
## Code to generate follow-up input1:
```java
    int year1 = 1990;
    int half1 = 2;
    int year2 = 1995;
    int year3 = year1;
    int half3 = half1;
```
Explanation: The inferred relation is that the result of `YearHalf.of(year1, half1).with(Year.of(year2))` should be equal to `YearHalf.of(year3, half3)`. Since `year1` and `year2` are the same, the result of `Year.of(year2)` is also the same as `Year.of(year1)`, so the inferred relation is satisfied.

# New input pair2:
```java
    int year1 = 2050;
    int half1 = 1;
    int year2 = 2055;
    int year3 = 2055;
    int half3 = 1;
```
## Code to generate follow-up input2:
```java
    int year1 = 2050;
    int half1 = 1;
    int year2 = 2055;
    int year3 = year1;
    int half3 = half1;
```
Explanation: The inferred relation is that the result of `YearHalf.of(year1, half1).with(Year.of(year2))` should be equal to `YearHalf.of(year3, half3)`. Since `year1` and `year2` are the same, the result of `Year.of(year2)` is also the same as `Year.of(year1)`, so the inferred relation is satisfied.

# New input pair3:
```java
    int year1 = 2100;
    int half1 = 2;
    int year2 = 2105;
    int year3 = 2105;
    int half3 = 2;
```
## Code to generate follow-up input3:
```java
    int year1 = 2100;
    int half1 = 2;
    int year2 = 2105;
    int year3 = year1;
    int half3 = half1;
```
Explanation: The inferred relation is that the result of `YearHalf.of(year1, half1).with(Year.of(year2))` should be equal to `YearHalf.of(year3, half3)`. Since `year1` and `year2` are the same, the result of `Year.of(year2)` is also the same as `Year.of(year1)`, so the inferred relation is satisfied.

# New input pair4:
```java
    int year1 = 2000;
    int half1 = 1;
    int year2 = 2000;
    int year3 = 2000;
    int half3 = 1;
```
## Code to generate follow-up input4:
```java
    int year1 = 2000;
    int half1 = 1;
    int year2 = 2000;
    int year3 = year1;
    int half3 = half1;
```
Explanation: The inferred relation is that the result of `YearHalf.of(year1, half1).with(Year.of(year2))` should be equal to `YearHalf.of(year3, half3)`. Since `year1` and `year2` are the same, the result of `Year.of(year2)` is also the same as `Year.of(year1)`, so the inferred relation is satisfied.
