## New input pair0:
```java
    Long value = 0L;
    String message = encrypt(value);
    Class<?> clazz = Long.class;
```
Explanation:
The inferred relation is that the encrypted value of a Long value can be decrypted back to the original value. Since the value is 0L, the encrypted value will also be 0L. Therefore, the follow-up input satisfies the inferred relation.

## New input pair1:
```java
    Long value = Long.MAX_VALUE;
    String message = encrypt(value);
    Class<?> clazz = Long.class;
```
Explanation:
The inferred relation is that the encrypted value of a Long value can be decrypted back to the original value. Since the value is Long.MAX_VALUE, the encrypted value will also be Long.MAX_VALUE. Therefore, the follow-up input satisfies the inferred relation.

## New input pair2:
```java
    Long value = Long.MIN_VALUE;
    String message = encrypt(value);
    Class<?> clazz = Long.class;
```
Explanation:
The inferred relation is that the encrypted value of a Long value can be decrypted back to the original value. Since the value is Long.MIN_VALUE, the encrypted value will also be Long.MIN_VALUE. Therefore, the follow-up input satisfies the inferred relation.

## New input pair3:
```java
    Long value = -1L;
    String message = encrypt(value);
    Class<?> clazz = Long.class;
```
Explanation:
The inferred relation is that the encrypted value of a Long value can be decrypted back to the original value. Since the value is -1L, the encrypted value will also be -1L. Therefore, the follow-up input satisfies the inferred relation.

## New input pair4:
```java
    Long value = 100L;
    String message = encrypt(value);
    Class<?> clazz = Long.class;
```
Explanation:
The inferred relation is that the encrypted value of a Long value can be decrypted back to the original value. Since the value is 100L, the encrypted value will also be 100L. Therefore, the follow-up input satisfies the inferred relation.
