## New input pair0:
```java
    NameState nameState = new NameState();
    NameState nextNameState = new NameState();
    String key = "key1";
    String key2 = "key1";
    NameState nameState2 = nameState;
    nameState.addNextNameState(key, nextNameState);
    assertEquals(nextNameState, nameState2.getNextNameState(key2));
```

## New input pair1:
```java
    NameState nameState = new NameState();
    NameState nextNameState = new NameState();
    String key = "key2";
    String key2 = "key2";
    NameState nameState2 = nameState;
    nameState.addNextNameState(key, nextNameState);
    assertEquals(nextNameState, nameState2.getNextNameState(key2));
```

## New input pair2:
```java
    NameState nameState = new NameState();
    NameState nextNameState = new NameState();
    String key = "";
    String key2 = "";
    NameState nameState2 = nameState;
    nameState.addNextNameState(key, nextNameState);
    assertEquals(nextNameState, nameState2.getNextNameState(key2));
```

## New input pair3:
```java
    NameState nameState = new NameState();
    NameState nextNameState = null;
    String key = "key";
    String key2 = "key";
    NameState nameState2 = nameState;
    nameState.addNextNameState(key, nextNameState);
    assertNull(nameState2.getNextNameState(key2));
```

## New input pair4:
```java
    NameState nameState = new NameState();
    NameState nextNameState = new NameState();
    String key = "key";
    String key2 = "key";
    NameState nameState2 = nameState;
    nextNameState.addNextNameState(key, nextNameState);
    nameState.addNextNameState(key, nextNameState);
    assertEquals(nextNameState, nameState2.getNextNameState(key2));
```

Explanation:
The inferred relation is that the `getNextNameState` method returns the `nextNameState` associated with the given `key` in the `nameState` object. The `addNextNameState` method adds a new `nextNameState` for the given `key` in the `nameState` object.

For the first new input pair, we create a new `NameState` object, add a new `nextNameState` for the key "key1" and then retrieve it using the same key. The expected result is that the retrieved `nextNameState` is the same as the added `nextNameState`.

For the second new input pair, we create a new `NameState` object, add a new `nextNameState` for the key "key2" and then retrieve it using the same key. The expected result is that the retrieved `nextNameState` is the same as the added `nextNameState`.

For the third new input pair, we create a new `NameState` object, add a new `nextNameState` for an empty key and then retrieve it using the same empty key. The expected result is that the retrieved `nextNameState` is the same as the added `nextNameState`.

For the fourth new input pair, we create a new `NameState` object, set the `nextNameState` to null, add a new `nextNameState` for the key "key" and then retrieve it using the same key. The expected result is that the retrieved `nextNameState` is null.

For the fifth new input pair, we create a new `NameState` object, add a new `nextNameState` for the key "key" and then add another `nextNameState` for the same key. The expected result is that the retrieved `nextNameState` is the same as the added `nextNameState` after the second addition.
