## New input pair0:
```java
    int year1 = 2020;
    int half1 = 1;
    int year2 = 2024;
    int year3 = 2024;
    int half3 = 1;
```
### Code to generate follow-up input:
```java
    int year1 = 2020;
    int half1 = 1;
    int year2 = 2024;
    int year3 = YearHalf.of(year1, half1).with(Year.of(year2)).getYear();
    int half3 = YearHalf.of(year1, half1).with(Year.of(year2)).getHalf().getValue();
```
### Explanation:
The inferred relation is that the result of `YearHalf.of(year1, half1).with(Year.of(year2))` should be equal to `YearHalf.of(year3, half3)`. Since `year3` is the result of applying the `with` method to `YearHalf.of(year1, half1)` with `Year.of(year2)`, and `half3` is the result of applying the `getHalf` method to the same `YearHalf`, the new input pair satisfies the inferred relation.

## New input pair1:
```java
    int year1 = 1900;
    int half1 = 2;
    int year2 = 1904;
    int year3 = 1904;
    int half3 = 2;
```
### Code to generate follow-up input:
```java
    int year1 = 1900;
    int half1 = 2;
    int year2 = 1904;
    int year3 = YearHalf.of(year1, half1).with(Year.of(year2)).getYear();
    int half3 = YearHalf.of(year1, half1).with(Year.of(year2)).getHalf().getValue();
```
### Explanation:
The inferred relation is that the result of `YearHalf.of(year1, half1).with(Year.of(year2))` should be equal to `YearHalf.of(year3, half3)`. Since `year3` is the result of applying the `with` method to `YearHalf.of(year1, half1)` with `Year.of(year2)`, and `half3` is the result of applying the `getHalf` method to the same `YearHalf`, the new input pair satisfies the inferred relation.

## New input pair2:
```java
    int year1 = 2000;
    int half1 = 1;
    int year2 = 2004;
    int year3 = 2004;
    int half3 = 1;
```
### Code to generate follow-up input:
```java
    int year1 = 2000;
    int half1 = 1;
    int year2 = 2004;
    int year3 = YearHalf.of(year1, half1).with(Year.of(year2)).getYear();
    int half3 = YearHalf.of(year1, half1).with(Year.of(year2)).getHalf().getValue();
```
### Explanation:
The inferred relation is that the result of `YearHalf.of(year1, half1).with(Year.of(year2))` should be equal to `YearHalf.of(year3, half3)`. Since `year3` is the result of applying the `with` method to `YearHalf.of(year1, half1)` with `Year.of(year2)`, and `half3` is the result of applying the `getHalf` method to the same `YearHalf`, the new input pair satisfies the inferred relation.

## New input pair3:
```java
    int year1 = 2100;
    int half1 = 2;
    int year2 = 2104;
    int year3 = 2104;
    int half3 = 2;
```
### Code to generate follow-up input:
```java
    int year1 = 2100;
    int half1 = 2;
    int year2 = 2104;
    int year3 = YearHalf.of(year1, half1).with(Year.of(year2)).getYear();
    int half3 = YearHalf.of(year1, half1).with(Year.of(year2)).getHalf().getValue();
```
### Explanation:
The inferred relation is that the result of `YearHalf.of(year1, half1).with(Year.of(year2))` should be equal to `YearHalf.of(year3, half3)`. Since `year3` is the result of applying the `with` method to `YearHalf.of(year1, half1)` with `Year.of(year2)`, and `half3` is the result of applying the `getHalf` method to the same `YearHalf`, the new input pair satisfies the inferred relation.

## New input pair4:
```java
    int year1 = 1800;
    int half1 = 1;
    int year2 = 1804;
    int year3 = 1804;
    int half3 = 1;
```
### Code to generate follow-up input:
```java
    int year1 = 1800;
    int half1 = 1;
    int year2 = 1804;
    int year3 = YearHalf.of(year1, half1).with(Year.of(year2)).getYear();
    int half3 = YearHalf.of(year1, half1).with(Year.of(year2)).getHalf().getValue();
```
### Explanation:
The inferred relation is that the result of `YearHalf.of(year1, half1).with(Year.of(year2))` should be equal to `YearHalf.of(year3, half3)`. Since `year3` is the result of applying the `with` method to `YearHalf.of(year1, half1)` with `Year.of(year2)`, and `half3` is the result of applying the `getHalf` method to the same `YearHalf`, the new input pair satisfies the inferred relation.
