# New input pair0:
```java
    int year1 = 2020;
    int half1 = 1;
    int half2 = 2;
    int year3 = 2020;
    int half3 = 2;
```
## Code to generate follow-up input0:
```java
    int year1 = 2020;
    int half1 = 1;
    int half2 = 2;
    int year3 = YearHalf.of(year1, half1).withHalf(half2).getYear();
    int half3 = YearHalf.of(year1, half1).withHalf(half2).getHalf().getValue();
```
Explanation: The inferred relation is that `YearHalf.of(year1, half1).withHalf(half2)` should return a `YearHalf` object with the same year and half as `YearHalf.of(year3, half3)`. Therefore, to satisfy this relation, we need to set `year3` to the year of the result of `YearHalf.of(year1, half1).withHalf(half2)` and `half3` to the half of the result of `YearHalf.of(year1, half1).withHalf(half2)`.

# New input pair1:
```java
    int year1 = 1900;
    int half1 = 2;
    int half2 = 1;
    int year3 = 1900;
    int half3 = 1;
```
## Code to generate follow-up input1:
```java
    int year1 = 1900;
    int half1 = 2;
    int half2 = 1;
    int year3 = YearHalf.of(year1, half1).withHalf(half2).getYear();
    int half3 = YearHalf.of(year1, half1).withHalf(half2).getHalf().getValue();
```
Explanation: The inferred relation is that `YearHalf.of(year1, half1).withHalf(half2)` should return a `YearHalf` object with the same year and half as `YearHalf.of(year3, half3)`. Therefore, to satisfy this relation, we need to set `year3` to the year of the result of `YearHalf.of(year1, half1).withHalf(half2)` and `half3` to the half of the result of `YearHalf.of(year1, half1).withHalf(half2)`.

# New input pair2:
```java
    int year1 = 2100;
    int half1 = 1;
    int half2 = 2;
    int year3 = 2100;
    int half3 = 2;
```
## Code to generate follow-up input2:
```java
    int year1 = 2100;
    int half1 = 1;
    int half2 = 2;
    int year3 = YearHalf.of(year1, half1).withHalf(half2).getYear();
    int half3 = YearHalf.of(year1, half1).withHalf(half2).getHalf().getValue();
```
Explanation: The inferred relation is that `YearHalf.of(year1, half1).withHalf(half2)` should return a `YearHalf` object with the same year and half as `YearHalf.of(year3, half3)`. Therefore, to satisfy this relation, we need to set `year3` to the year of the result of `YearHalf.of(year1, half1).withHalf(half2)` and `half3` to the half of the result of `YearHalf.of(year1, half1).withHalf(half2)`.

# New input pair3:
```java
    int year1 = 2000;
    int half1 = 2;
    int half2 = 1;
    int year3 = 2000;
    int half3 = 1;
```
## Code to generate follow-up input3:
```java
    int year1 = 2000;
    int half1 = 2;
    int half2 = 1;
    int year3 = YearHalf.of(year1, half1).withHalf(half2).getYear();
    int half3 = YearHalf.of(year1, half1).withHalf(half2).getHalf().getValue();
```
Explanation: The inferred relation is that `YearHalf.of(year1, half1).withHalf(half2)` should return a `YearHalf` object with the same year and half as `YearHalf.of(year3, half3)`. Therefore, to satisfy this relation, we need to set `year3` to the year of the result of `YearHalf.of(year1, half1).withHalf(half2)` and `half3` to the half of the result of `YearHalf.of(year1, half1).withHalf(half2)`.

# New input pair4:
```java
    int year1 = 2007;
    int half1 = 1;
    int half2 = 1;
    int year3 = 2007;
    int half3 = 1;
```
## Code to generate follow-up input4:
```java
    int year1 = 2007;
    int half1 = 1;
    int half2 = 1;
    int year3 = YearHalf.of(year1, half1).withHalf(half2).getYear();
    int half3 = YearHalf.of(year1, half1).withHalf(half2).getHalf().getValue();
```
Explanation: The inferred relation is that `YearHalf.of(year1, half1).withHalf(half2)` should return a `YearHalf` object with the same year and half as `YearHalf.of(year3, half3)`. Therefore, to satisfy this relation, we need to set `year3` to the year of the result of `YearHalf.of(year1, half1).withHalf(half2)` and `half3` to the half of the result of `YearHalf.of(year1, half1).withHalf(half2)`.
