# REQUIRED DELIVERABLE
## New input pair0:
```java
    int year1 = 1900;
    int half1 = 1;
    int half2 = 2;
    int year3 = 1900;
    int half3 = 2;
```
### Code to generate follow-up input:
```java
    int year1 = 1900;
    int half1 = 1;
    int half2 = 2;
    int year3 = YearHalf.of(year1, half1).withHalf(half2).getYear();
    int half3 = YearHalf.of(year1, half1).withHalf(half2).getHalf().getValue();
```
### Explanation:
The inferred relation is that the result of `YearHalf.of(year1, half1).withHalf(half2)` should be equal to `YearHalf.of(year3, half3)`. Since `year1` is 1900, `half1` is 1, and `half2` is 2, the result of `YearHalf.of(year1, half1).withHalf(half2)` is `YearHalf.of(1900, 2)`. The `getYear()` method returns the year, which is 1900, and the `getHalf().getValue()` method returns the half-of-year, which is 2. Therefore, the result of `YearHalf.of(year3, half3)` is `YearHalf.of(1900, 2)`, which is equal to the result of `YearHalf.of(year1, half1).withHalf(half2)`.

## New input pair1:
```java
    int year1 = 2100;
    int half1 = 2;
    int half2 = 1;
    int year3 = 2100;
    int half3 = 1;
```
### Code to generate follow-up input:
```java
    int year1 = 2100;
    int half1 = 2;
    int half2 = 1;
    int year3 = YearHalf.of(year1, half1).withHalf(half2).getYear();
    int half3 = YearHalf.of(year1, half1).withHalf(half2).getHalf().getValue();
```
### Explanation:
The inferred relation is that the result of `YearHalf.of(year1, half1).withHalf(half2)` should be equal to `YearHalf.of(year3, half3)`. Since `year1` is 2100, `half1` is 2, and `half2` is 1, the result of `YearHalf.of(year1, half1).withHalf(half2)` is `YearHalf.of(2100, 1)`. The `getYear()` method returns the year, which is 2100, and the `getHalf().getValue()` method returns the half-of-year, which is 1. Therefore, the result of `YearHalf.of(year3, half3)` is `YearHalf.of(2100, 1)`, which is equal to the result of `YearHalf.of(year1, half1).withHalf(half2)`.

## New input pair2:
```java
    int year1 = 2000;
    int half1 = 1;
    int half2 = 2;
    int year3 = 2000;
    int half3 = 2;
```
### Code to generate follow-up input:
```java
    int year1 = 2000;
    int half1 = 1;
    int half2 = 2;
    int year3 = YearHalf.of(year1, half1).withHalf(half2).getYear();
    int half3 = YearHalf.of(year1, half1).withHalf(half2).getHalf().getValue();
```
### Explanation:
The inferred relation is that the result of `YearHalf.of(year1, half1).withHalf(half2)` should be equal to `YearHalf.of(year3, half3)`. Since `year1` is 2000, `half1` is 1, and `half2` is 2, the result of `YearHalf.of(year1, half1).withHalf(half2)` is `YearHalf.of(2000, 2)`. The `getYear()` method returns the year, which is 2000, and the `getHalf().getValue()` method returns the half-of-year, which is 2. Therefore, the result of `YearHalf.of(year3, half3)` is `YearHalf.of(2000, 2)`, which is equal to the result of `YearHalf.of(year1, half1).withHalf(half2)`.

## New input pair3:
```java
    int year1 = 2000;
    int half1 = 2;
    int half2 = 1;
    int year3 = 2000;
    int half3 = 1;
```
### Code to generate follow-up input:
```java
    int year1 = 2000;
    int half1 = 2;
    int half2 = 1;
    int year3 = YearHalf.of(year1, half1).withHalf(half2).getYear();
    int half3 = YearHalf.of(year1, half1).withHalf(half2).getHalf().getValue();
```
### Explanation:
The inferred relation is that the result of `YearHalf.of(year1, half1).withHalf(half2)` should be equal to `YearHalf.of(year3, half3)`. Since `year1` is 2000, `half1` is 2, and `half2` is 1, the result of `YearHalf.of(year1, half1).withHalf(half2)` is `YearHalf.of(2000, 1)`. The `getYear()` method returns the year, which is 2000, and the `getHalf().getValue()` method returns the half-of-year, which is 1. Therefore, the result of `YearHalf.of(year3, half3)` is `YearHalf.of(2000, 1)`, which is equal to the result of `YearHalf.of(year1, half1).withHalf(half2)`.

## New input pair4:
```java
    int year1 = 1800;
    int half1 = 1;
    int half2 = 2;
    int year3 = 1800;
    int half3 = 2;
```
### Code to generate follow-up input:
```java
    int year1 = 1800;
    int half1 = 1;
    int half2 = 2;
    int year3 = YearHalf.of(year1, half1).withHalf(half2).getYear();
    int half3 = YearHalf.of(year1, half1).withHalf(half2).getHalf().getValue();
```
### Explanation:
The inferred relation is that the result of `YearHalf.of(year1, half1).withHalf(half2)` should be equal to `YearHalf.of(year3, half3)`. Since `year1` is 1800, `half1` is 1, and `half2` is 2, the result of `YearHalf.of(year1, half1).withHalf(half2)` is `YearHalf.of(1800, 2)`. The `getYear()` method returns the year, which is 1800, and the `getHalf().getValue()` method returns the half-of-year, which is 2. Therefore, the result of `YearHalf.of(year3, half3)` is `YearHalf.of(1800, 2)`, which is equal to the result of `YearHalf.of(year1, half1).withHalf(half2)`.
