# METHOD UNDER TEST
```java
public static IsFalseDimFilter of(DimFilter field) {
    return new IsFalseDimFilter(field);
}

```


# TEST CASE
```java
@Test
public void testGetCacheKey() {
    EqualityFilter f3 = new EqualityFilter("x", ColumnType.STRING, "hello", null);
    EqualityFilter f4 = new EqualityFilter("x", ColumnType.STRING, "hello", null);
    IsFalseDimFilter f1_3 = IsFalseDimFilter.of(f3);
    IsFalseDimFilter f1_4 = IsFalseDimFilter.of(f4);
    Assert.assertArrayEquals(f1_3.getCacheKey(), f1_4.getCacheKey());
}

```
SOURCE INPUT: `f3`
FOLLOW UP INPUT: `f4`


# OTHER INPUT PAIRS 
## Input pair1:
```java
EqualityFilter f3 = new EqualityFilter("x", ColumnType.STRING, "hello", null);
EqualityFilter f4 = new EqualityFilter("x", ColumnType.STRING, "hello", null);
```

## Input pair2:
```java
EqualityFilter f3 = new EqualityFilter("x", ColumnType.STRING, "", null);
EqualityFilter f4 = new EqualityFilter("x", ColumnType.STRING, "", null);
```

## Input pair3:
```java
EqualityFilter f3 = new EqualityFilter("x", ColumnType.STRING, "123", null);
EqualityFilter f4 = new EqualityFilter("x", ColumnType.STRING, "123", null);
```

## Input pair4:
```java
EqualityFilter f3 = new EqualityFilter("y", ColumnType.STRING, "hello", null);
EqualityFilter f4 = new EqualityFilter("y", ColumnType.STRING, "hello", null);
```

## Input pair5:
```java
EqualityFilter f3 = new EqualityFilter("x", ColumnType.LONG, 123, null);
EqualityFilter f4 = new EqualityFilter("x", ColumnType.LONG, 123, null);
```

## Input pair6:
```java
EqualityFilter f3 = new EqualityFilter("x", ColumnType.STRING, "world", null);
EqualityFilter f4 = new EqualityFilter("x", ColumnType.STRING, "world", null);
```



# OUTPUT FORMAT
```java
public class IsBooleanDimFilterTest_testGetCacheKey {
    public static EqualityFilter inputTransformation_testGetCacheKey(EqualityFilter f3)  {
        // TODO
        EqualityFilter f4 = 
		return f4;
    }
}
```
Your task is to deduce the relationship between 'SOURCE INPUT' and 'FOLLOW UP INPUT' in the test case, and create a function that transforms 'SOURCE INPUT' into 'FOLLOW UP INPUT'.
The deduced relation and generated transformation function should be applicable to addtional input pairs and other potentail input pairs with similar characteristics.
Generate the transformation function by complementing the above code skeleton in 'OUTPUT FORMAT'.