## New input pair0:
```java
    NameState nameState = new NameState();
    NameState nextNameState = new NameState();
    String key = "";
    String key2 = "";
    NameState nameState2 = nameState;
```

Explanation: 
In the original test case, the `key` and `key2` are both empty strings. The `addNextNameState` method adds the `nextNameState` to the `nameState` using the `key` as the key in the `keyToNextNameState` map. The `getNextNameState` method retrieves the value from the `keyToNextNameState` map using the `key2`. Since both `key` and `key2` are empty strings, they are considered equal and the `nextNameState` is returned. Therefore, in the new input pair, we can use empty strings for both `key` and `key2` to satisfy the inferred relation.

## New input pair1:
```java
    NameState nameState = new NameState();
    NameState nextNameState = null;
    String key = "key";
    String key2 = "key";
    NameState nameState2 = nameState;
```

Explanation: 
In the original test case, the `key` and `key2` are both "key". The `addNextNameState` method adds the `nextNameState` to the `nameState` using the `key` as the key in the `keyToNextNameState` map. The `getNextNameState` method retrieves the value from the `keyToNextNameState` map using the `key2`. Since both `key` and `key2` are equal, the `nextNameState` is returned. Therefore, in the new input pair, we can use "key" for both `key` and `key2` to satisfy the inferred relation. Additionally, we can set `nextNameState` to `null` to test the behavior when the value associated with the key is `null`.

## New input pair2:
```java
    NameState nameState = new NameState();
    NameState nextNameState = new NameState();
    String key = "key2";
    String key2 = "key2";
    NameState nameState2 = nameState;
```

Explanation: 
In the original test case, the `key` and `key2` are both "key2". The `addNextNameState` method adds the `nextNameState` to the `nameState` using the `key` as the key in the `keyToNextNameState` map. The `getNextNameState` method retrieves the value from the `keyToNextNameState` map using the `key2`. Since both `key` and `key2` are equal, the `nextNameState` is returned. Therefore, in the new input pair, we can use "key2" for both `key` and `key2` to satisfy the inferred relation.

## New input pair3:
```java
    NameState nameState = new NameState();
    NameState nextNameState = new NameState();
    String key = "key";
    String key2 = "key";
    NameState nameState2 = nameState;
```

Explanation: 
This is the same as the original source input pair. We can reuse the original source input pair to satisfy the inferred relation.